updates to STac including some proofs.
- Proofs for tactic combinators but not for
  "real" tactics.

theories/STac/Core.v
@@ -11,16 +11,30 @@ Set Strict Implicit.
 Section parameterized.
   Variable typ : Type.
   Variable expr : Type.
-  (** TODO: I'm going to need to thread facts for a prover through here **)
+  (** TODO: I might want some way to maintain external state **)
   Variable subst : Type.
 
   Inductive Result : Type :=
   | Fail
-  | Solve : subst -> Result
-  | Progress : expr -> subst -> list typ -> list typ -> Result.
+  | Solved : subst -> Result
+  | More : list typ -> list typ -> subst -> expr -> Result.
 
   Definition stac : Type :=
-    expr -> subst -> list typ -> list typ ->
+    (** TODO: Part of the state is hypotheses **)
+    list typ -> list typ -> subst -> expr ->
     Result.
+
+  Axiom goalD : forall (tus tvs : list typ) (s : subst) (goal : expr), Prop.
+
+  Definition stac_sound (tac : stac) : Prop
+  := forall tus tvs s (g : expr),
+       match tac tus tvs s g with
+         | Fail => True
+         | Solved s' =>
+           goalD tus tvs s g (* /\ Extends s' s *)
+         | More tus' tvs' s' g' =>
+           goalD tus' tvs' s' g' ->
+           goalD tus tvs s g
+       end.
 
 End parameterized.
