theories/STac/Simplify.v
@@ -9,10 +9,20 @@ Section parameterized.
   Variable subst : Type.
 
   Definition SIMPLIFY
-             (f : list typ -> list typ -> expr -> expr)
-             (thn : stac typ expr subst)
+             (f : list typ -> list typ -> subst -> expr -> expr)
   : stac typ expr subst :=
-    fun e s tus tvs =>
-      thn (f tus tvs e) s tus tvs.
+    fun tus tvs s e =>
+      More tus tvs s (f tus tvs s e).
+
+  Theorem SIMPLIFY_sound
+  : forall f,
+      (forall tus tvs s e e',
+         f tus tvs s e = e' ->
+         goalD tus tvs s e' -> goalD tus tvs s e) ->
+      stac_sound (SIMPLIFY f).
+  Proof.
+    intros. unfold stac_sound, SIMPLIFY.
+    intros. eapply H. reflexivity. eauto.
+  Qed.
 
 End parameterized.
