theories/STac/Solve.v
@@ -11,8 +11,15 @@ Section parameterized.
   Definition SOLVE (b : stac typ expr subst) : stac typ expr subst :=
     fun e sub tus tvs =>
       match b e sub tus tvs with
-        | Solve s => @Solve _ _ _ s
+        | Solved s => @Solved _ _ _ s
         | x => @Fail _ _ _
       end.
+
+  Theorem SOLVE_sound : forall t, stac_sound t -> stac_sound (SOLVE t).
+  Proof.
+    unfold stac_sound; simpl; intros.
+    red. specialize (H tus tvs s g).
+    destruct (t tus tvs s g); auto.
+  Qed.
 
 End parameterized.
