theories/STac/Try.v
@@ -9,10 +9,17 @@ Section parameterized.
   Variable subst : Type.
 
   Definition TRY (b : stac typ expr subst) : stac typ expr subst :=
-    fun e sub tus tvs =>
-      match b e sub tus tvs with
-        | Fail => Progress e sub tus tvs
+    fun tus tvs sub e =>
+      match b tus tvs sub e with
+        | Fail => More tus tvs sub e
         | x => x
       end.
+
+  Theorem TRY_sound : forall b, stac_sound b -> stac_sound (TRY b).
+  Proof.
+    unfold stac_sound; intros.
+    specialize (H tus tvs s g). unfold TRY.
+    destruct (b tus tvs s g); auto.
+  Qed.
 
 End parameterized.
